# Generalized Stirling Transform

## Classical Stirling Transform

The classical Stirling transform relates polynomial sequences through Stirling numbers:

- For Stirling numbers of the first kind $s(n,k)$:
  $x^{\underline{n}} = \sum_{k=0}^{n} s(n,k) x^k$ (expressing falling factorials in terms of powers)

- For Stirling numbers of the second kind $S(n,k)$:
  $x^n = \sum_{k=0}^{n} S(n,k) x^{\underline{k}}$ (expressing powers in terms of falling factorials)

These transforms are inverses of each other, allowing conversion between different polynomial bases.

## Generalized Stirling Transform with Inverse Functions

We can generalize this concept using the generalized Stirling numbers $S_{n,k}(a,b)$ and two functions $f$ and $g$ that are inverses of each other.

### Definition

Given two inverse functions $f$ and $g$ (where $f(g(x)) = g(f(x)) = x$), the generalized Stirling transform can be expressed as:

$$f(x)^n = \sum_{k=0}^{n} S_{n,k}(a,b) [g(x)]^{\underline{k}}$$

and its inverse:

$$[g(x)]^{\underline{n}} = \sum_{k=0}^{n} s_{n,k}(a,b) f(x)^k$$

where $S_{n,k}(a,b)$ and $s_{n,k}(a,b)$ are generalized Stirling numbers with parameters $a$ and $b$.

### Properties

1. **Duality**: The transform maintains the duality relationship between the generalized Stirling numbers of the first and second kind.

2. **Basis Transformation**: This provides a way to transform between different functional bases in polynomial spaces.

3. **Parameter Dependence**: The specific values of $a$ and $b$ determine how the bases are related and the characteristics of the transformation.

### Examples

- When $f(x) = x$ and $g(x) = x$, with $(a,b) = (0,1)$ or $(a,b) = (1,0)$, we recover the classical Stirling transforms.

- For $f(x) = e^x$ and $g(x) = \ln(x)$, we get exponential generating functions and Bell-like transforms.

- For $f(x) = \frac{1}{1-x}$ and $g(x) = \frac{x}{1+x}$, we obtain transforms related to ordinary generating functions.

## Applications

This generalized transform framework allows:

1. Conversion between various polynomial bases beyond the standard power and factorial bases
2. Development of efficient algorithms for polynomial manipulations
3. Analysis of combinatorial structures through different functional perspectives
4. Creation of specialized transforms for specific problem domains by selecting appropriate function pairs and parameters

## Mathematical Challenges

Open questions include:

1. Determining which function pairs $(f,g)$ yield closed-form expressions for the transform coefficients
2. Understanding how the parameters $(a,b)$ affect the convergence properties of the transform
3. Developing efficient computational methods for applying these transforms to large datasets

## Inverse Relationships in Exponential Generating Functions

### Theoretical Foundation

**Theorem 1:** *For any pair of compositionally inverse functions with exponential generating functions, there exists a specific parameter pair $(a,b)$ for which the generalized Stirling numbers transform the coefficient sequence of one function to that of its inverse.*

Let $f(x) = \sum_{m=0}^{\infty} a_m \frac{x^m}{m!}$ and $g(x) = \sum_{m=0}^{\infty} b_m \frac{x^m}{m!}$ be two exponential generating functions where $g$ behaves as a functional inverse of $f$ (i.e., $g(f(x)) \approx x$). Then the coefficients $\{b_n\}$ can be derived from $\{a_m\}$ via the transformation:

$$b_n = \sum_{k=0}^{n} S_{n,k}(a,b) \cdot a_k$$

where $S_{n,k}(a,b)$ are the generalized Stirling numbers with specific parameters $(a,b)$ that depend on the functional relationship.

*Proof:* For functional inverses, we must have:
$$g(f(x)) = x$$

Expanding the left side:
$$b_0 + b_1 f(x) + \frac{b_2}{2!}[f(x)]^2 + \cdots = x$$

Substituting the series for $f(x)$ and equating coefficients of $x^n$, we obtain constraints that determine the relationship between $\{a_m\}$ and $\{b_n\}$. This relationship follows the structure of generalized Stirling transformations.

The specific parameter $b$ can be approximated using the second-order terms:
$$b \approx -\frac{a_2 b_1^2 - a_1^2 b_2}{a_1^2 b_1}$$

For normalized functions with $a_0=b_0=0$ and $a_1=b_1=1$, this simplifies to $b \approx a_2-b_2$.

### Classic Example: Exponential and Logarithm

For the classic inverse pair:
- $f(x) = e^{rx} - 1 = rx + \frac{r^2x^2}{2!} + \cdots$
- $g(x) = \frac{1}{r}\ln(1+x) = \frac{x}{r} - \frac{x^2}{2r} + \frac{x^3}{3r} - \cdots$

We have $a_0 = 0$, $a_1 = r$, $a_2 = r^2$, and $b_0 = 0$, $b_1 = \frac{1}{r}$, $b_2 = -\frac{1}{2r}$

Applying the parameter estimation formula:
$$b \approx -\frac{r^2 \cdot (1/r)^2 - r^2 \cdot (-1/2r)}{r^2 \cdot (1/r)} = -1 + \frac{1}{2} = -\frac{1}{2}$$

The exact value is $b = -1$, with the approximation improving as we consider higher-order terms.

This corresponds to Stirling numbers of the first kind with parameters $(a,b)=(1,-1)$.

### Extended Examples

#### Hyperbolic Functions

For hyperbolic sine and its inverse:
- $f(x) = \sinh(x) = x + \frac{x^3}{3!} + \frac{x^5}{5!} + \cdots$
- $g(x) = \text{arsinh}(x) = x - \frac{1}{2}\frac{x^3}{3} + \frac{1 \cdot 3}{2 \cdot 4}\frac{x^5}{5} - \cdots$

The transformation between these series involves parameters approximately $(a,b) \approx (0,-\frac{1}{2})$, reflecting the specific curvature properties of these functions.

#### Rational Functions

For rational functions:
- $f(x) = \frac{x}{1-x} = x + x^2 + x^3 + \cdots$
- $g(x) = \frac{x}{1+x} = x - x^2 + x^3 - \cdots$

These alternating coefficients are related through parameters $(a,b) \approx (0,-1)$.

#### Laguerre Polynomials

The generalized Laguerre polynomials $L_n^{(\alpha)}(x)$ have the EGF:
$$\sum_{n=0}^{\infty} L_n^{(\alpha)}(x) \frac{t^n}{n!} = \frac{e^{-xt/(1-t)}}{(1-t)^{\alpha+1}}$$

Their connection to generalized Stirling numbers comes through the umbral calculus, where:
$$L_n^{(\alpha)}(x) = \sum_{k=0}^{n} \binom{n+\alpha}{n-k} \frac{(-x)^k}{k!}$$

This expansion can be interpreted using generalized Stirling numbers with parameters $(a,b)$ depending on $\alpha$.

#### Touchard Polynomials

The Touchard polynomials (also called exponential polynomials) $T_n(x)$ have the EGF:
$$\sum_{n=0}^{\infty} T_n(x) \frac{t^n}{n!} = e^{x(e^t-1)}$$

They satisfy:
$$T_n(x) = \sum_{k=0}^{n} S(n,k) x^k$$

where $S(n,k)$ are the Stirling numbers of the second kind. This is a special case of the generalized Stirling transform with parameters $(a,b) = (0,1)$.

#### Bell Polynomials

The complete Bell polynomials $B_n(x_1,x_2,\ldots,x_n)$ can be connected to generalized Stirling numbers through:
$$B_n(1!a_1, 2!a_2, \ldots, n!a_n) = n! \sum_{k=0}^{n} S_{n,k}(a,b) \frac{a_k}{k!}$$

for specific values of $(a,b)$ that depend on the sequence $\{a_n\}$.
$$[g^{-1}(x)]^{\underline{n}} = \sum_{k=0}^{n} s_{n,k}(a,b) [f^{-1}(x)]^k$$

where $s_{n,k}(a,b)$ are the generalized Stirling numbers of the first kind.

This approach provides a systematic way to determine the parameter $b$ that makes two EGFs functionally inverse through the lens of generalized Stirling transformations.
