# Hasse Operator and Generalized Stieltjes Constants

## 1. Introduction

This document establishes a profound connection between the Hasse shift operator and the generalized Stieltjes constants. We will show that the full Hasse operator applied to powers of the natural logarithm, `[log(x)]^k`, yields the generalized Stieltjes constants, up to a simple factor. This provides a new "summation" formula for these important number-theoretic constants.

## 2. Definitions

### 2.1 Generalized Stieltjes Constants

The Hurwitz zeta function, $\zeta(s,x)$, has a Laurent series expansion around its simple pole at $s=1$:

$$\zeta(s,x) = \frac{1}{s-1} + \sum_{k=0}^{\infty} \frac{(-1)^k \gamma_k(x)}{k!} (s-1)^k$$

The coefficients $\gamma_k(x)$ are the **generalized Stieltjes constants**. The classical Stieltjes constants are $\gamma_k = \gamma_k(1)$.

### 2.2 The Full Hasse Shift Operator

The full Hasse shift operator, $\mathcal{H}$, applied to a function $f$ is defined as the infinite sum over all orders $m$:

$$\mathcal{H}(f)(x) = \sum_{m=0}^{\infty} \mathcal{H}_m(f)(x) = \sum_{m=0}^{\infty} \sum_{n=0}^{m} H_{m,n} f(x+n)$$

## 3. The Main Connection Theorem

**Theorem:** The full Hasse shift operator applied to the k-th power of the natural logarithm is directly related to the (k-1)-th generalized Stieltjes constant.

$$\mathcal{H}([\log(t)]^k)(x) = (-1)^k k \cdot \gamma_{k-1}(x)$$

for $k \geq 1$.

## 4. Proof of the Theorem

The proof relies on a key identity connecting the Hasse operator to the Hurwitz zeta function, and then comparing two different series expansions for the same quantity.

**Step 1: The Hasse-Hurwitz Identity**

We start with the known identity:
$$(s-1)\zeta(s,x) = \mathcal{H}(t \mapsto t^{1-s})(x)$$
This identity states that the function $(s-1)\zeta(s,x)$ (as a function of $x$) is equal to the Hasse operator applied to the function $f(t) = t^{1-s}$.

**Step 2: Laurent Series of the Left-Hand Side**

From the definition of the generalized Stieltjes constants, we can write the series for the left-hand side around $s=1$:
$$(s-1)\zeta(s,x) = 1 + \sum_{k=1}^{\infty} \frac{(-1)^k \gamma_k(x)}{k!} (s-1)^{k+1} = 1 + \sum_{k=1}^{\infty} \frac{(-1)^{k-1} \gamma_{k-1}(x)}{(k-1)!} (s-1)^k$$

**Step 3: Taylor Series of the Right-Hand Side**

Now, we expand the function inside the Hasse operator on the right-hand side as a Taylor series in $(s-1)$:
$$t^{1-s} = e^{(1-s)\log(t)} = \sum_{k=0}^{\infty} \frac{(\log t)^k (1-s)^k}{k!} = \sum_{k=0}^{\infty} \frac{(-1)^k (\log t)^k}{k!} (s-1)^k$$

Applying the Hasse operator $\mathcal{H}$ (which is linear) term-by-term:
$$\mathcal{H}(t \mapsto t^{1-s})(x) = \mathcal{H}\left(\sum_{k=0}^{\infty} \frac{(-1)^k (\log t)^k}{k!} (s-1)^k\right)(x)$$
$$= \sum_{k=0}^{\infty} \frac{(-1)^k (s-1)^k}{k!} \mathcal{H}((\log t)^k)(x)$$

**Step 4: Equating Coefficients**

We now have two power series in $(s-1)$ for the same function. By equating the coefficients of $(s-1)^k$, we can establish our result.

- **For k=0 (constant term):**
  - LHS: $1$
  - RHS: $\frac{(-1)^0}{0!} \mathcal{H}((\log t)^0)(x) = \mathcal{H}(1)(x) = 1$. This matches.

- **For k $\geq$ 1:**
  - LHS coefficient of $(s-1)^k$: $\frac{(-1)^{k-1} \gamma_{k-1}(x)}{(k-1)!}$
  - RHS coefficient of $(s-1)^k$: $\frac{(-1)^k}{k!} \mathcal{H}((\log t)^k)(x)$

Setting them equal:
$$\frac{(-1)^{k-1} \gamma_{k-1}(x)}{(k-1)!} = \frac{(-1)^k}{k!} \mathcal{H}((\log t)^k)(x)$$

Solving for $\mathcal{H}((\log t)^k)(x)$:
$$\mathcal{H}((\log t)^k)(x) = \frac{k!}{(k-1)!} \frac{(-1)^{k-1}}{(-1)^k} \gamma_{k-1}(x)$$
$$\mathcal{H}((\log t)^k)(x) = k \cdot (-1) \cdot \gamma_{k-1}(x) = (-k) \gamma_{k-1}(x)$$
This seems to have a sign error from the prompt's intuition. Let's re-check the Laurent series.

Ah, the standard definition is:
$\zeta(s,x) = \frac{1}{s-1} + \sum_{n=0}^{\infty} \frac{(-1)^n \gamma_n(x)}{n!} (s-1)^n$.
Then $(s-1)\zeta(s,x) = 1 + \sum_{n=0}^{\infty} \frac{(-1)^n \gamma_n(x)}{n!} (s-1)^{n+1}$.
Let $k=n+1$, so $n=k-1$.
$(s-1)\zeta(s,x) = 1 + \sum_{k=1}^{\infty} \frac{(-1)^{k-1} \gamma_{k-1}(x)}{(k-1)!} (s-1)^k$. This is correct.

Let's re-check the final algebra.
$$\frac{(-1)^{k-1} \gamma_{k-1}(x)}{(k-1)!} = \frac{(-1)^k}{k!} \mathcal{H}([\log t]^k)(x)$$
$$\mathcal{H}([\log t]^k)(x) = \frac{k!}{(k-1)!} \frac{(-1)^{k-1}}{(-1)^k} \gamma_{k-1}(x) = k \cdot (-1) \cdot \gamma_{k-1}(x)$$
The derivation seems to lead to a factor of `-k`. Let's assume this is correct for now.

**Corrected Theorem:**
$$\mathcal{H}([\log(t)]^k)(x) = -k \cdot \gamma_{k-1}(x)$$

## 5. Implications and Conclusion

This theorem is remarkable. It provides a completely new representation for the generalized Stieltjes constants, defining them not by a limit or an integral, but as the result of an infinite discrete summation operator applied to a fundamental function.

- **Computational Tool**: This identity can be used as a method to numerically approximate the Stieltjes constants by truncating the infinite sum of the Hasse operator.
- **Theoretical Insight**: It reveals a deep structural link between the analytic behavior of the zeta function near its pole and the combinatorial properties of discrete difference operators.
- **Generalization**: This framework connects the entire family of Stieltjes constants ($\gamma_0, \gamma_1, \ldots$) to the family of logarithmic powers ($[\log t]^1, [\log t]^2, \ldots$) via a single, unified operator.
