# The Hasse Operator: A Unified Approach

## 1. Definition of Hasse Coefficients

The Hasse coefficients, denoted by $H_{m,n}$, form the foundation of the Hasse operator theory. They are defined as:

$$H_{m,n} = \frac{(-1)^n \binom{m}{n}}{m+1}$$

where $\binom{m}{n}$ is the binomial coefficient and $0 \leq n \leq m$.

**Key properties**:
- For $m \geq 1$: $\sum_{n=0}^{m} H_{m,n} = 0$ (normalization property)
- $H_{0,0} = 1$ (base case)
- $H_{m,n} = 0$ for $n > m$ (domain restriction)
- For fixed $m$, the sequence $\{H_{m,n}\}_{n=0}^{m}$ alternates in sign

The Hasse coefficients satisfy a useful recurrence relation:

$$H_{m+1,n} = H_{m,n-1} - \frac{m+1-n}{m+2} \cdot H_{m,n}$$

for $1 \leq n \leq m+1$, with boundary condition $H_{m,0} = \frac{1}{m+1}$.

## 2. The Hasse Shift Operator

The Hasse shift operator is defined in terms of these coefficients. For a function $f(x)$, the $m$-th order Hasse operator is:

$$\mathcal{H}_m(f)(x) = \sum_{n=0}^{m} H_{m,n} f(x+n)$$

This represents a weighted average of shifted values of $f$, with weights given by the Hasse coefficients.

The full Hasse operator is the infinite sum of all orders:

$$\mathcal{H}(f)(x) = \sum_{m=0}^{\infty} \mathcal{H}_m(f)(x)$$

For well-behaved functions, this infinite sum converges and reveals profound connections to special functions.

## 3. Relationship to Shift and Finite Difference Operators

### 3.1 Shift Operator Representation

Let $E$ denote the shift operator: $E f(x) = f(x+1)$. Powers of $E$ represent multiple shifts: $E^n f(x) = f(x+n)$.

The Hasse operator can be expressed as a weighted sum of shift operators:

$$\mathcal{H}_m = \frac{1}{m+1} \sum_{k=0}^{m} (-1)^k \binom{m}{k} E^k$$

This representation shows that the Hasse operator is a specific linear combination of shifts.

### 3.2 Connection to Finite Differences

The forward difference operator $\Delta$ is defined as $\Delta f(x) = f(x+1) - f(x) = (E-I)f(x)$, where $I$ is the identity operator.

Since $\Delta = E - I$, we can express the shift operator as $E = I + \Delta$. Substituting this into the Hasse operator expression:

$$\mathcal{H}_m = \frac{1}{m+1} \sum_{k=0}^{m} (-1)^k \binom{m}{k} (I + \Delta)^k$$

Using the binomial theorem:

$$\mathcal{H}_m = \frac{1}{m+1} \sum_{k=0}^{m} (-1)^k \binom{m}{k} \sum_{j=0}^{k} \binom{k}{j} \Delta^j$$

Rearranging:

$$\mathcal{H}_m = \frac{1}{m+1} \sum_{j=0}^{m} \Delta^j \sum_{k=j}^{m} (-1)^k \binom{m}{k} \binom{k}{j}$$

The inner sum relates to Stirling numbers of the first kind, giving:

$$\mathcal{H}_m = \frac{1}{m+1} \sum_{j=0}^{m} s(m,j) \frac{\Delta^j}{j!}$$

where $s(m,j)$ are the (unsigned) Stirling numbers of the first kind.

This demonstrates that the Hasse operator can be viewed as a specific combination of finite difference operators of various orders.

## 4. Action on Basic Functions

Let's examine how the Hasse operator acts on simple functions.

### 4.1 Constant Functions

For $f(x) = 1$:
- $\mathcal{H}_0(1) = H_{0,0} \cdot 1 = 1$
- For $m \geq 1$: $\mathcal{H}_m(1) = \sum_{n=0}^{m} H_{m,n} = 0$ (by the normalization property)

Therefore, $\mathcal{H}(1) = 1$.

### 4.2 Linear Functions

For $f(x) = x$:
- $\mathcal{H}_0(x) = H_{0,0} \cdot x = x$
- $\mathcal{H}_1(x) = H_{1,0} \cdot x + H_{1,1} \cdot (x+1) = \frac{1}{2}x - \frac{1}{2}(x+1) = -\frac{1}{2}$
- For $m \geq 2$: $\mathcal{H}_m(x)$ can be shown to equal 0

Therefore, $\mathcal{H}(x) = x - \frac{1}{2}$.

### 4.3 Quadratic Functions

For $f(x) = x^2$:
- $\mathcal{H}_0(x^2) = H_{0,0} \cdot x^2 = x^2$
- $\mathcal{H}_1(x^2) = H_{1,0} \cdot x^2 + H_{1,1} \cdot (x+1)^2 = \frac{1}{2}x^2 - \frac{1}{2}(x^2+2x+1) = -\frac{1}{2}(2x+1)$
- $\mathcal{H}_2(x^2) = H_{2,0} \cdot x^2 + H_{2,1} \cdot (x+1)^2 + H_{2,2} \cdot (x+2)^2$
  $= \frac{1}{3}x^2 - \frac{2}{3}(x^2+2x+1) + \frac{1}{3}(x^2+4x+4) = \frac{1}{6}$
- For $m \geq 3:
