# Product Analysis: $S_{m,n}(a,0) \cdot S_{m,n}(0,b)$

## Overview

This document analyzes the product of two specific types of generalized Stirling transfer coefficients: $S_{m,n}(a,0)$ (transforming from generalized factorial with increment $a$ to monomials) and $S_{m,n}(0,b)$ (transforming from monomials to generalized factorial with increment $b$).

## Individual Scaling Relationships

From our established results:

### $S_{m,n}(a,0)$ - Factorial to Monomial
$$S_{m,n}(a,0) = a^{m-n} \left\{\begin{array}{c}m\\n\end{array}\right\}$$

### $S_{m,n}(0,b)$ - Monomial to Factorial  
$$S_{m,n}(0,b) = b^{-n} s(m,n)$$

## Direct Product Analysis

### Product Formula
$$S_{m,n}(a,0) \cdot S_{m,n}(0,b) = a^{m-n} \left\{\begin{array}{c}m\\n\end{array}\right\} \cdot b^{-n} s(m,n)$$

$$= a^{m-n} b^{-n} \left\{\begin{array}{c}m\\n\end{array}\right\} s(m,n)$$

$$= \left(\frac{a}{b}\right)^{m-n} a^{-n} b^{-n} \left\{\begin{array}{c}m\\n\end{array}\right\} s(m,n)$$

$$= \left(\frac{a}{b}\right)^m (ab)^{-n} \left\{\begin{array}{c}m\\n\end{array}\right\} s(m,n)$$

### Classical Orthogonality Factor

The key insight is that $\left\{\begin{array}{c}m\\n\end{array}\right\} s(m,n)$ involves the classical orthogonality relationship:

$$\sum_{k=0}^{m} \left\{\begin{array}{c}m\\k\end{array}\right\} s(k,n) = [m=n]$$

However, our product involves $\left\{\begin{array}{c}m\\n\end{array}\right\} s(m,n)$ directly, not the orthogonal sum.

## Matrix Product Interpretation

### Matrix Formulation

Consider the matrices:
- $\mathbf{A}(a,0)$ with entries $S_{m,n}(a,0) = a^{m-n} \left\{\begin{array}{c}m\\n\end{array}\right\}$
- $\mathbf{B}(0,b)$ with entries $S_{m,n}(0,b) = b^{-n} s(m,n)$

The **element-wise product** (Hadamard product) $\mathbf{A} \circ \mathbf{B}$ has entries:
$$(\mathbf{A} \circ \mathbf{B})_{m,n} = S_{m,n}(a,0) \cdot S_{m,n}(0,b) = \left(\frac{a}{b}\right)^m (ab)^{-n} \left\{\begin{array}{c}m\\n\end{array}\right\} s(m,n)$$

### Matrix Multiplication vs. Element-wise Product

**Important distinction:** This is NOT the same as matrix multiplication $\mathbf{A} \cdot \mathbf{B}$, which would give:
$$(\mathbf{A} \cdot \mathbf{B})_{m,n} = \sum_{k=0}^{m} S_{m,k}(a,0) \cdot S_{k,n}(0,b)$$

The matrix product corresponds to the composition transformation $S_{m,n}(a,b)$, while the element-wise product gives us a different mathematical object.

## Special Cases and Numerical Examples

### Case 1: $a = b = 1$

$$S_{m,n}(1,0) \cdot S_{m,n}(0,1) = \left\{\begin{array}{c}m\\n\end{array}\right\} s(m,n)$$

**Numerical values:**
- $S_{2,1}(1,0) \cdot S_{2,1}(0,1) = 1 \cdot (-1) = -1$
- $S_{3,2}(1,0) \cdot S_{3,2}(0,1) = 3 \cdot (-3) = -9$
- $S_{4,2}(1,0) \cdot S_{4,2}(0,1) = 7 \cdot 11 = 77$

### Case 2: $a = 2, b = 1$

$$S_{m,n}(2,0) \cdot S_{m,n}(0,1) = 2^{m-n} \left\{\begin{array}{c}m\\n\end{array}\right\} s(m,n)$$

**Numerical values:**
- $S_{2,1}(2,0) \cdot S_{2,1}(0,1) = 2^{2-1} \cdot 1 \cdot (-1) = 2 \cdot (-1) = -2$
- $S_{3,2}(2,0) \cdot S_{3,2}(0,1) = 2^{3-2} \cdot 3 \cdot (-3) = 2 \cdot (-9) = -18$

### Case 3: $a = 1, b = -1$

$$S_{m,n}(1,0) \cdot S_{m,n}(0,-1) = (-1)^{-n} \left\{\begin{array}{c}m\\n\end{array}\right\} \left[\begin{array}{c}m\\n\end{array}\right]$$

$$= (-1)^n \left\{\begin{array}{c}m\\n\end{array}\right\} \left[\begin{array}{c}m\\n\end{array}\right]$$

Since $\left[\begin{array}{c}m\\n\end{array}\right] = |s(m,n)|$, this gives:
$$= (-1)^n \left\{\begin{array}{c}m\\n\end{array}\right\} |s(m,n)|$$

## Diagonal Pattern Analysis

### Observation: Diagonal Structure

When we examine the element-wise product matrix, an interesting pattern emerges. For the classical case $a = b = 1$:

$$(\mathbf{A} \circ \mathbf{B})_{m,n} = \left\{\begin{array}{c}m\\n\end{array}\right\} s(m,n)$$

The orthogonality relationship suggests that while individual products $\left\{\begin{array}{c}m\\n\end{array}\right\} s(m,n)$ may be non-zero, their weighted sums have special structure.

### Diagonal Entries

For $m = n$:
$$S_{m,m}(a,0) \cdot S_{m,m}(0,b) = a^{m-m} \left\{\begin{array}{c}m\\m\end{array}\right\} \cdot b^{-m} s(m,m)$$

$$= 1 \cdot 1 \cdot b^{-m} \cdot 1 = b^{-m}$$

Since $\left\{\begin{array}{c}m\\m\end{array}\right\} = 1$ and $s(m,m) = 1$ always.

### Off-Diagonal Structure

For $m \neq n$, the products involve non-trivial Stirling number combinations with scaling factors.

## Connection to Generalized Stirling Coefficients

### Relationship to $S_{m,n}(a,b)$

The element-wise product is **not** equal to $S_{m,n}(a,b)$. Instead:

$$S_{m,n}(a,b) = \sum_{k=0}^{m} S_{m,k}(a,0) \cdot S_{k,n}(0,b)$$

This is the matrix multiplication formula, which gives the actual transformation coefficients.

### Verification Through Composition

For $a = 1, b = -1$:
$$S_{m,n}(1,-1) = \sum_{k=0}^{m} S_{m,k}(1,0) \cdot S_{k,n}(0,-1)$$

$$= \sum_{k=0}^{m} \left\{\begin{array}{c}m\\k\end{array}\right\} \cdot (-1)^n k^{-n} \left[\begin{array}{c}k\\n\end{array}\right]$$

This composition gives the Lah number relationship:
$$S_{m,n}(1,-1) = (-1)^{m-n} L(m,n)$$

## Generating Function Analysis

### Element-wise Product Generating Function

Consider the generating function of the element-wise products:

$$\sum_{m,n=0}^{\infty} S_{m,n}(a,0) \cdot S_{m,n}(0,b) \frac{x^m y^n}{m! n!}$$

$$= \sum_{m,n=0}^{\infty} \left(\frac{a}{b}\right)^m (ab)^{-n} \left\{\begin{array}{c}m\\n\end{array}\right\} s(m,n) \frac{x^m y^n}{m! n!}$$

This can be related to the generating functions of individual Stirling numbers:

$$\sum_{m=0}^{\infty} \left\{\begin{array}{c}m\\n\end{array}\right\} \frac{x^m}{m!} = \frac{(e^x - 1)^n}{n!}$$

$$\sum_{m=0}^{\infty} s(m,n) \frac{x^m}{m!} = \frac{(\log(1+x))^n}{n!}$$

## Combinatorial Interpretation

### Meaning of the Product

The product $S_{m,n}(a,0) \cdot S_{m,n}(0,b)$ can be interpreted as:

1. **$S_{m,n}(a,0)$**: Ways to convert an $a$-factorial of degree $m$ into monomials of degree $n$
2. **$S_{m,n}(0,b)$**: Ways to convert monomials of degree $m$ into $b$-factorials of degree $n$

The **element-wise product** counts something different from the **composition** (matrix product).

### Scaling Interpretation

The factor $\left(\frac{a}{b}\right)^m (ab)^{-n}$ provides scaling information:
- $\left(\frac{a}{b}\right)^m$: Relative scaling between source and target increment parameters
- $(ab)^{-n}$: Inverse scaling factor depending on target degree

## Applications and Future Directions

### Potential Applications

1. **Weighted combinatorial problems** where transformations have multiplicative costs
2. **Generating function manipulations** involving element-wise operations
3. **Statistical mechanics** models with competing scaling factors

### Research Questions

1. **Closed form** for the element-wise product generating function
2. **Asymptotic behavior** of products for large parameters
3. **Inverse problems** - when does the product have special structure?
4. **Generalization** to other coefficient pairs

## Summary

The element-wise product $S_{m,n}(a,0) \cdot S_{m,n}(0,b)$ yields:

$$\left(\frac{a}{b}\right)^m (ab)^{-n} \left\{\begin{array}{c}m\\n\end{array}\right\} s(m,n)$$

This is distinct from the composition $S_{m,n}(a,b)$ and has its own mathematical structure involving:
- **Scaling factors** from increment parameters
- **Classical Stirling number products** 
- **Diagonal dominance** in special cases
- **Generating function** connections to classical results

The analysis reveals how element-wise operations on generalized Stirling matrices create new mathematical objects with their own interesting properties and potential applications.
