### Recurrence Relations

The generalized Stirling transfer coefficients satisfy recurrence relations derived from the properties of generalized factorial polynomials:

$$S_{m+1,n}(a,b) = S_{m,n-1}(a,b) \cdot nb + S_{m,n}(a,b) \cdot (x + ma) \tag{17}$$

This recurrence follows from the fundamental recurrence of $P(x,a,m)$.

## Inductive Proof of General Form for $a \neq 0 \neq b$

### Conjecture

For $a \neq 0 \neq b$, the generalized Stirling transfer coefficients have the form:

$$S_{m,n}(a,b) = \sum_{k} \left[m \atop k\right] \cdot \left\{k \atop n\right\} \cdot (-b)^{f(m,n,k)} \cdot a^{g(m,n,k)} \tag{18}$$

where $\left[m \atop k\right]$ are Stirling numbers of the first kind, $\left\{k \atop n\right\}$ are Stirling numbers of the second kind, and we need to determine the power functions $f(m,n,k)$ and $g(m,n,k)$.

### Case Analysis

#### Case 1: Trivial Case (m=0 or n=0)

**Boundary conditions:**

- $S_{0,0}(a,b) = 1$ (identity transformation)
- $S_{m,0}(a,b) = 0$ for $m > 0$ when $a \neq 0$
- $S_{0,n}(a,b) = 0$ for $n > 0$

These match the boundary conditions of classical Stirling numbers, confirming the base case.

#### Case 2: 2×2 Matrix Analysis

Let's examine the transformation for $m,n \leq 2$:

**Target:** Find $S_{m,n}(a,b)$ for the 2×2 submatrix:
$$\begin{pmatrix}
S_{1,1}(a,b) & S_{1,2}(a,b) \\
S_{2,1}(a,b) & S_{2,2}(a,b)
\end{pmatrix}$$

**Step 1:** Express $P(x,a,1)$ and $P(x,a,2)$ in terms of $P(x,b,n)$

From the definition:
$$P(x,a,1) = x = S_{1,1}(a,b) \cdot P(x,b,1) + S_{1,2}(a,b) \cdot P(x,b,2)$$
$$P(x,a,2) = x(x+a) = S_{2,1}(a,b) \cdot P(x,b,1) + S_{2,2}(a,b) \cdot P(x,b,2)$$

where:
- $P(x,b,1) = x$
- $P(x,b,2) = x(x+b)$

**Step 2:** Solve the system

From the first equation:
$$x = S_{1,1}(a,b) \cdot x + S_{1,2}(a,b) \cdot x(x+b)$$

Comparing coefficients:
- Coefficient of $x$: $1 = S_{1,1}(a,b) + S_{1,2}(a,b) \cdot b$
- Coefficient of $x^2$: $0 = S_{1,2}(a,b)$

Therefore: $S_{1,2}(a,b) = 0$ and $S_{1,1}(a,b) = 1$.

From the second equation:
$$x^2 + ax = S_{2,1}(a,b) \cdot x + S_{2,2}(a,b) \cdot x(x+b)$$
$$x^2 + ax = S_{2,1}(a,b) \cdot x + S_{2,2}(a,b) \cdot (x^2 + bx)$$

Comparing coefficients:
- Coefficient of $x^2$: $1 = S_{2,2}(a,b)$
- Coefficient of $x$: $a = S_{2,1}(a,b) + S_{2,2}(a,b) \cdot b = S_{2,1}(a,b) + b$

Therefore: $S_{2,2}(a,b) = 1$ and $S_{2,1}(a,b) = a - b$.

**Step 3:** Pattern Analysis for 2×2 Case

The 2×2 matrix is:
$$\begin{pmatrix}
1 & 0 \\
a-b & 1
\end{pmatrix}$$

Let's check this against the classical Stirling forms:
- $\left[1 \atop 1\right] = 1$, $\left[2 \atop 1\right] = -1$, $\left[2 \atop 2\right] = 1$
- $\left\{1 \atop 1\right\} = 1$, $\left\{2 \atop 1\right\} = 1$, $\left\{2 \atop 2\right\} = 1$

**Pattern identification:**
- $S_{1,1}(a,b) = 1 = \left[1 \atop 1\right] \cdot \left\{1 \atop 1\right\} \cdot (-b)^0 \cdot a^0$
- $S_{2,1}(a,b) = a-b = -1 \cdot 1 \cdot (-b)^1 \cdot a^0 + 1 \cdot 1 \cdot (-b)^0 \cdot a^1$
- $S_{2,2}(a,b) = 1 = \left[2 \atop 2\right] \cdot \left\{2 \atop 2\right\} \cdot (-b)^0 \cdot a^0$

This suggests:
$$S_{2,1}(a,b) = \left[2 \atop 1\right] \cdot \left\{1 \atop 1\right\} \cdot (-b)^1 + \left[2 \atop 2\right] \cdot \left\{2 \atop 1\right\} \cdot a^1$$

#### Case 3: 3×3 Matrix Analysis

**Next step:** Compute $S_{3,n}(a,b)$ for $n = 1,2,3$.

From $P(x,a,3) = x(x+a)(x+2a) = x^3 + 3ax^2 + 2a^2x$:

$$x^3 + 3ax^2 + 2a^2x = S_{3,1}(a,b) \cdot x + S_{3,2}(a,b) \cdot x(x+b) + S_{3,3}(a,b) \cdot x(x+b)(x+2b)$$

Expanding the right side:
$$S_{3,1}(a,b) \cdot x + S_{3,2}(a,b) \cdot (x^2 + bx) + S_{3,3}(a,b) \cdot (x^3 + 3bx^2 + 2b^2x)$$

Comparing coefficients:
- $x^3$: $1 = S_{3,3}(a,b)$
- $x^2$: $3a = S_{3,2}(a,b) + 3b \cdot S_{3,3}(a,b) = S_{3,2}(a,b) + 3b$
- $x^1$: $2a^2 = S_{3,1}(a,b) + b \cdot S_{3,2}(a,b) + 2b^2 \cdot S_{3,3}(a,b)$

Solving:
- $S_{3,3}(a,b) = 1$
- $S_{3,2}(a,b) = 3a - 3b = 3(a-b)$
- $S_{3,1}(a,b) = 2a^2 - b(3a-3b) - 2b^2 = 2a^2 - 3ab + 3b^2 - 2b^2 = 2a^2 - 3ab + b^2$

### Symbolic Matrix Inversion Approach

**Alternative Method Using Matrix Algebra:**

Instead of coefficient comparison, we can use symbolic matrix inversion to find the transfer coefficients more systematically.

#### 2×2 Symbolic Inversion

The transformation system can be written as:
$$\begin{pmatrix} P(x,a,1) \\ P(x,a,2) \end{pmatrix} = \begin{pmatrix} S_{1,1}(a,b) & S_{1,2}(a,b) \\ S_{2,1}(a,b) & S_{2,2}(a,b) \end{pmatrix} \begin{pmatrix} P(x,b,1) \\ P(x,b,2) \end{pmatrix}$$

Let $\mathbf{A}_a = \begin{pmatrix} x \\ x(x+a) \end{pmatrix}$ and $\mathbf{A}_b = \begin{pmatrix} x \\ x(x+b) \end{pmatrix}$.

Then: $\mathbf{A}_a = \mathbf{S}_{2×2}(a,b) \cdot \mathbf{A}_b$

**Coefficient Matrix Method:**

From $\mathbf{A}_a$ and $\mathbf{A}_b$, extract coefficient matrices:
$$\mathbf{A}_a = \begin{pmatrix} 0 & 1 \\ a & 1 \end{pmatrix} \begin{pmatrix} 1 \\ x \end{pmatrix}, \quad \mathbf{A}_b = \begin{pmatrix} 0 & 1 \\ b & 1 \end{pmatrix} \begin{pmatrix} 1 \\ x \end{pmatrix}$$

Let $\mathbf{C}_a = \begin{pmatrix} 0 & 1 \\ a & 1 \end{pmatrix}$ and $\mathbf{C}_b = \begin{pmatrix} 0 & 1 \\ b & 1 \end{pmatrix}$.

Then: $\mathbf{S}_{2×2}(a,b) = \mathbf{C}_a \cdot \mathbf{C}_b^{-1}$

**Computing $\mathbf{C}_b^{-1}$ symbolically:**

For $\mathbf{C}_b = \begin{pmatrix} 0 & 1 \\ b & 1 \end{pmatrix}$:

- Determinant: $\det(\mathbf{C}_b) = 0 \cdot 1 - 1 \cdot b = -b$
- Adjugate: $\text{adj}(\mathbf{C}_b) = \begin{pmatrix} 1 & -1 \\ -b & 0 \end{pmatrix}$

Therefore:
$$\mathbf{C}_b^{-1} = \frac{1}{-b} \begin{pmatrix} 1 & -1 \\ -b & 0 \end{pmatrix} = \begin{pmatrix} -\frac{1}{b} & \frac{1}{b} \\ 1 & 0 \end{pmatrix}$$

**Computing the transfer matrix:**
$$\mathbf{S}_{2×2}(a,b) = \begin{pmatrix} 0 & 1 \\ a & 1 \end{pmatrix} \begin{pmatrix} -\frac{1}{b} & \frac{1}{b} \\ 1 & 0 \end{pmatrix} = \begin{pmatrix} 1 & 0 \\ a-b & 1 \end{pmatrix}$$

This confirms our previous result with pure symbolic manipulation.

#### 3×3 Symbolic Inversion

For the 3×3 case, we have:
$$\mathbf{C}_a = \begin{pmatrix} 0 & 0 & 1 \\ 0 & a & 1 \\ 2a^2 & 3a & 1 \end{pmatrix}, \quad \mathbf{C}_b = \begin{pmatrix} 0 & 0 & 1 \\ 0 & b & 1 \\ 2b^2 & 3b & 1 \end{pmatrix}$$

**Computing $\mathbf{C}_b^{-1}$ using symbolic methods:**

For a 3×3 matrix $\begin{pmatrix} 0 & 0 & 1 \\ 0 & b & 1 \\ 2b^2 & 3b & 1 \end{pmatrix}$:

- Determinant (expanding along first row): $\det(\mathbf{C}_b) = 1 \cdot \det\begin{pmatrix} 0 & b \\ 2b^2 & 3b \end{pmatrix} = 1 \cdot (0 \cdot 3b - b \cdot 2b^2) = -2b^3$

Using cofactor expansion for the adjugate matrix:
$$\text{adj}(\mathbf{C}_b) = \begin{pmatrix} b^2-3b & 3b & -b \\ 2b^2 & -2b^2 & 0 \\ -2b^3 & 0 & 0 \end{pmatrix}^T = \begin{pmatrix} b^2-3b & 2b^2 & -2b^3 \\ 3b & -2b^2 & 0 \\ -b & 0 & 0 \end{pmatrix}$$

Therefore:
$$\mathbf{C}_b^{-1} = \frac{1}{-2b^3} \begin{pmatrix} b^2-3b & 2b^2 & -2b^3 \\ 3b & -2b^2 & 0 \\ -b & 0 & 0 \end{pmatrix}$$

**Transfer matrix calculation:**
$$\mathbf{S}_{3×3}(a,b) = \mathbf{C}_a \cdot \mathbf{C}_b^{-1}$$

This systematic approach using symbolic matrix algebra provides:
1. **Exact symbolic expressions** without numerical approximation
2. **Systematic verification** of coefficient patterns
3. **Scalable methodology** for higher-order cases
4. **Direct connection** to linear algebra theory

**Advantages of Symbolic Approach:**

- **No coefficient matching errors**: Direct matrix operations eliminate transcription mistakes  
- **Pattern recognition**: Matrix structure reveals underlying algebraic relationships
- **Inverse verification**: Can check $\mathbf{S}(a,b) \cdot \mathbf{S}(b,a) = \mathbf{I}$ symbolically
- **Computational efficiency**: Symbolic computation systems handle the algebra automatically

### Pattern Recognition

From the computations above, let's identify the pattern:

Looking at our results:

- $S_{1,1}(a,b) = 1$
- $S_{2,1}(a,b) = a - b$  
- $S_{2,2}(a,b) = 1$
- $S_{3,1}(a,b) = 2a^2 - 3ab + b^2$
- $S_{3,2}(a,b) = 3(a-b)$
- $S_{3,3}(a,b) = 1$

**Analysis using classical Stirling numbers:**

Recall:
- $\left[2 \atop 1\right] = -1$, $\left[2 \atop 2\right] = 1$
- $\left[3 \atop 1\right] = 2$, $\left[3 \atop 2\right] = -3$, $\left[3 \atop 3\right] = 1$
- $\left\{1 \atop 1\right\} = 1$, $\left\{2 \atop 1\right\} = 1$, $\left\{2 \atop 2\right\} = 1$, $\left\{3 \atop 1\right\} = 1$, $\left\{3 \atop 2\right\} = 3$, $\left\{3 \atop 3\right\} = 1$

**Pattern Hypothesis:**

From the examples, it appears that:

$$S_{m,n}(a,b) = \sum_{k=0}^{\min(m,n)} \left[m \atop k\right] \cdot \left\{k \atop n\right\} \cdot a^{m-k} \cdot (-b)^{n-k} \tag{20}$$

**Verification Status:**

Initial tests of this formula against computed values show discrepancies, indicating the pattern requires refinement. The key issue is that the simple product form doesn't capture all the scaling relationships observed in specific cases like Lah numbers.

**Lah Numbers Verification Case:**

Let's also verify our pattern against the known Lah number case: $S_{m,n}(1,-1) = (-1)^{m-n} L(m,n)$.

From the main article, we know:
- $L(1,1) = 1$
- $L(2,1) = 2$, $L(2,2) = 1$  
- $L(3,1) = 6$, $L(3,2) = 6$, $L(3,3) = 1$

So we should have:
- $S_{1,1}(1,-1) = (-1)^{1-1} L(1,1) = 1 \cdot 1 = 1$
- $S_{2,1}(1,-1) = (-1)^{2-1} L(2,1) = (-1) \cdot 2 = -2$
- $S_{2,2}(1,-1) = (-1)^{2-2} L(2,2) = 1 \cdot 1 = 1$
- $S_{3,1}(1,-1) = (-1)^{3-1} L(3,1) = 1 \cdot 6 = 6$
- $S_{3,2}(1,-1) = (-1)^{3-2} L(3,2) = (-1) \cdot 6 = -6$
- $S_{3,3}(1,-1) = (-1)^{3-3} L(3,3) = 1 \cdot 1 = 1$

**Testing Pattern Hypothesis with Lah Numbers:**

Using our conjectured form (20a) with $a = 1, b = -1$:

For $S_{2,1}(1,-1) = -2$:
$$S_{2,1}(1,-1) = \frac{1^2}{(-(-1))^1} \sum_{k=0}^{1} \left[2 \atop k\right] \cdot \left\{k \atop 1\right\} \cdot \left(\frac{-(-1)}{1}\right)^k$$

$$= \frac{1}{1} \left[ \left[2 \atop 0\right] \cdot \left\{0 \atop 1\right\} \cdot 1 + \left[2 \atop 1\right] \cdot \left\{1 \atop 1\right\} \cdot 1 \right]$$

$$= 1 \left[ 0 \cdot 0 + (-1) \cdot 1 \cdot 1 \right] = -1$$

This gives $-1$ instead of $-2$, confirming our pattern needs refinement.

For $S_{3,2}(1,-1) = -6$:
$$S_{3,2}(1,-1) = \frac{1^3}{(-(-1))^2} \sum_{k=0}^{2} \left[3 \atop k\right] \cdot \left\{k \atop 2\right\} \cdot \left(\frac{1}{1}\right)^k$$

$$= \frac{1}{1} \left[ \left[3 \atop 0\right] \cdot \left\{0 \atop 2\right\} + \left[3 \atop 1\right] \cdot \left\{1 \atop 2\right\} + \left[3 \atop 2\right] \cdot \left\{2 \atop 2\right\} \right]$$

$$= 1 \left[ 0 \cdot 0 + 2 \cdot 0 + (-3) \cdot 1 \right] = -3$$

This gives $-3$ instead of $-6$.

**Pattern Recognition Enhancement:**

The Lah number verification shows that our current pattern is missing scaling factors. Notice that:
- Expected: $S_{2,1}(1,-1) = -2$, Got: $-1$ (factor of 2 missing)
- Expected: $S_{3,2}(1,-1) = -6$, Got: $-3$ (factor of 2 missing)

This suggests the correct pattern might involve additional multiplicative factors related to the indices.

**Fresh Approach - Direct Pattern Analysis:**

Let me examine the computed values more carefully:

- $S_{1,1}(a,b) = 1$
- $S_{2,1}(a,b) = a - b$
- $S_{2,2}(a,b) = 1$  
- $S_{3,1}(a,b) = 2a^2 - 3ab + b^2$
- $S_{3,2}(a,b) = 3(a-b)$
- $S_{3,3}(a,b) = 1$

Notice that:
- $S_{2,1}(a,b) = a - b = 1 \cdot a^1 \cdot b^0 + (-1) \cdot a^0 \cdot b^1$
- $S_{3,1}(a,b) = 2a^2 - 3ab + b^2 = 2 \cdot a^2 \cdot b^0 + (-3) \cdot a^1 \cdot b^1 + 1 \cdot a^0 \cdot b^2$
- $S_{3,2}(a,b) = 3(a-b) = 3 \cdot a^1 \cdot b^0 + (-3) \cdot a^0 \cdot b^1$

**Pattern Recognition:**

The coefficients appear to be multinomial-like expansions. Let me conjecture:

$$S_{m,n}(a,b) = \sum_{j=0}^{n} c_{m,n,j} \cdot a^{n-j} \cdot b^j \tag{20c}$$

where the $c_{m,n,j}$ coefficients are combinations of Stirling numbers with bracket notation:

$$c_{m,n,j} = \sum_{k} \left[m \atop k\right] \cdot \left\{k \atop n\right\} \cdot [\text{appropriate combinatorial factor}] \tag{20d}$$

**Lah Numbers as Pattern Guide:**

The Lah number relationship $S_{m,n}(1,-1) = (-1)^{m-n} L(m,n)$ provides crucial insight. Since Lah numbers are defined as:

$$L(m,n) = \binom{m-1}{n-1} \frac{m!}{n!} = \frac{m!}{n!(n-1)!(m-n)!} \cdot (m-1)!$$

And they satisfy:
$$L(m,n) = \sum_{k=0}^{\min(m,n)} \left[m \atop k\right] \cdot \left\{k \atop n\right\} \cdot \text{[scaling factor]}$$


where $f(a,b,m,n,k)$ captures the appropriate scaling and alternating sign patterns observed in the Lah case.

**Inductive Strategy Using Lah Numbers:**

1. **Base verification**: Confirm pattern works for known Lah cases
2. **Parameter scaling**: Use $a=1, b=-1$ to isolate the Stirling product structure  
3. **General scaling**: Extend to arbitrary $a,b$ using scaling inheritance
4. **Inductive step**: Prove the recurrence relation preserves the pattern

**Analysis Framework:**

The key insight is that we need to match:
1. The triangular structure (upper triangular zeros)
2. The diagonal elements (all equal to 1)
3. The sub-diagonal pattern involving $(a-b)$ terms

This suggests the form should respect both the $a$ and $b$ scaling while maintaining the classical Stirling number relationships in the coefficients $c_{m,n,j}$.

### Inductive Framework


Using the recurrence relation (17), we need to show:
$$S_{m+1,n}(a,b) = S_{m,n-1}(a,b) \cdot nb + S_{m,n}(a,b) \cdot (ma)$$

satisfies our conjectured form.

**Next Steps:**

1. **Lah Number Verification**: Use the known $S_{m,n}(1,-1) = (-1)^{m-n} L(m,n)$ relationship to determine the correct scaling factors in the Stirling product formula
2. **Precise Coefficient Determination**: Identify the exact form of $f(a,b,m,n,k)$ using Lah numbers as a guide
3. **Multi-case Verification**: Test the refined formula against all computed 2×2, 3×3, and Lah number cases
4. **Inductive Proof**: Use the recurrence relation to prove the pattern holds for all $m,n$
5. **Classical Limit Verification**: Confirm reduction to classical Stirling numbers when $a=0,b=1$ or $a=1,b=0$

The Lah numbers provide a crucial "Rosetta Stone" for decoding the general pattern, since they represent a specific, well-understood case of the generalized Stirling transfer coefficients with known explicit formulas.

## Unit Circle Property of Classical Stirling Numbers

**Observation**: Most conventional Stirling number cases correspond to parameters lying on the unit circle in the complex plane, since they involve combinations of $0, \pm 1$.

**Classical Cases on Unit Circle:**

1. **Stirling First Kind**: $S_{m,n}(0,1) \rightarrow |a/b| = |0/1| = 0$ (origin)
2. **Stirling Second Kind**: $S_{m,n}(1,0) \rightarrow |a/b| = |1/0| = \infty$ (point at infinity)  
3. **Lah Numbers**: $S_{m,n}(1,-1) \rightarrow |a/b| = |1/(-1)| = 1$ (unit circle)
4. **Unsigned Stirling**: $S_{m,n}(0,-1) \rightarrow |a/b| = |0/(-1)| = 0$ (origin)
5. **Modified Second Kind**: $S_{m,n}(-1,0) \rightarrow |a/b| = |(-1)/0| = \infty$ (point at infinity)
6. **Inverse Lah**: $S_{m,n}(-1,1) \rightarrow |a/b| = |(-1)/1| = 1$ (unit circle)

**Geometric Interpretation:**

The unit circle cases $(a,b) = (1,-1)$ and $(a,b) = (-1,1)$ correspond to **pure rotational transformations** in the parameter space, while cases involving $0$ correspond to **scaling degeneracies** (origin or infinity).

This suggests that:
- **Unit circle cases** preserve certain structural properties (like the connection to Lah numbers)
- **Degenerate cases** ($a=0$ or $b=0$) reduce to classical Stirling numbers
- **General cases** $(|a/b| \neq 0,1,\infty)$ require the full generalized framework

## Left Coset Structure (Notes to be Recovered)

**Conjecture**: The generalized Stirling transfer coefficients may have an underlying **left coset structure** in some appropriate group or algebraic framework.

**Preliminary Ideas:**
- The parameter transformations $(a,b) \mapsto (ka, kb)$ for $k \neq 0$ preserve certain structural relationships
- The inverse relationships $S_{m,n}(a,b) \leftrightarrow S_{m,n}(b,a)$ suggest a group-like structure
- Classical cases may correspond to coset representatives

**Next Steps for Algebraic Framework:**
1. **Recover detailed notes** on left coset construction
2. **Identify the underlying group** acting on parameter pairs $(a,b)$
3. **Establish coset representatives** for equivalence classes
4. **Connect to known representation theory** of symmetric groups or related structures

This algebraic perspective could provide the missing theoretical foundation for the inductive proof and explain why the pattern involves products of $\left[m \atop k\right]$ and $\left\{k \atop n\right\}$ with specific scaling factors.
